src/proofs/block_common/properties_block_common_functions.dfy
@@ -1,8 +1,8 @@
-include "../../common/block_proposal/block_types.dfy"
-include "../../common/block_proposal/block_common_functions.dfy"
+include "../../common/block_proposer/block_types.dfy"
+include "../../common/block_proposer/block_common_functions.dfy"
 
-import opened BlockTypes
-import opened BlockCommonFunctions
+import opened Block_Types
+import opened Block_Common_Functions
 
 lemma {:axiom} compute_domain_properties(dom1 : DomainTypes, ep1: Epoch, dom2: DomainTypes, ep2: Epoch)
 requires compute_domain(dom1, ep1) == compute_domain(dom2, ep2) 
