src/proofs/no_slashable_blocks/supporting_lemmas/dv_next_preserves_ind_inv/invs_fnc_1.dfy
@@ -1,12 +1,12 @@
 include "../../../../common/commons.dfy"
-include "../../common/block_proposal_instrumented.dfy"
+include "../../common/block_proposer_instrumented.dfy"
 include "../../../../specs/consensus/consensus.dfy"
 include "../../../../specs/network/network.dfy"
 include "../../../../specs/dv/dv_attestation_creation.dfy"
 include "../inv.dfy"
 include "../../../common/helper_sets_lemmas.dfy"
 include "../../common/common_proofs.dfy"
-include "../../common/dvc_spec_axioms_for_blocks.dfy"
+include "../../common/block_dvc_spec_axioms.dfy"
 
 include "../../../common/helper_pred_fcn.dfy"
 
